tuned more proofs

src/HOL/Nominal/Examples/Fsub.thy
@@ -4,35 +4,47 @@ theory fsub
 imports "../nominal" 
 begin
 
-text {* Authors: Christian Urban
-                 Benjamin Pierce
-                 Steve Zdancewic
-                 Stephanie Weihrich
-                 Dimitrios Vytiniotis
+text {* Authors: Christian Urban,
+                 Benjamin Pierce,
+                 Steve Zdancewic.
+                 Stephanie Weihrich and
+                 Dimitrios Vytiniotis;
 
-                 with help from Stefan Berghofer, Markus Wenzel
+                 with help from Stefan Berghofer and  Markus Wenzel.
       *}
 
 
+section {* Atom Types, Types and Terms *}
+
 atom_decl tyvrs vrs
 
-section {* Types *}
+nominal_datatype ty = 
+    TVar  "tyvrs"
+  | Top
+  | Arrow  "ty" "ty"          ("_ \<rightarrow> _" [900,900] 900)
+  | TAll  "\<guillemotleft>tyvrs\<guillemotright>ty" "ty" 
 
-nominal_datatype ty = TyVar "tyvrs"
-                    | Top
-                    | Arrow  "ty" "ty"          ("_ \<rightarrow> _" [900,900] 900)
-                    | TAll  "\<guillemotleft>tyvrs\<guillemotright>ty" "ty" 
+nominal_datatype trm = 
+    Var   "vrs"
+  | Lam   "\<guillemotleft>vrs\<guillemotright>trm" "ty"
+  | TAbs  "\<guillemotleft>tyvrs\<guillemotright>trm" "ty"
+  | App   "trm" "trm"
+  | TApp  "trm" "ty"
 
 syntax
   TAll_syn  :: "tyvrs \<Rightarrow> ty \<Rightarrow> ty \<Rightarrow> ty" ("\<forall> [_<:_]._" [900,900,900] 900)
-translations 
-  "(\<forall>[a<:ty1].ty2)" \<rightleftharpoons> "TAll a ty2 ty1"
+  Lam_syn   :: "vrs \<Rightarrow> ty \<Rightarrow> trm \<Rightarrow> trm"   ("Lam [_:_]._" [100,100,100] 100)
+  TAbs_syn  :: "tyvrs \<Rightarrow> ty \<Rightarrow> trm \<Rightarrow> trm" ("TAbs [_<:_]._" [100,100,100] 100)
 
-section {* typing contexts and their domains *}
+translations 
+  "\<forall>[a<:ty1].ty2" \<rightleftharpoons> "TAll a ty2 ty1"
+  "Lam  [a:tys].t" \<rightleftharpoons> "trm.Lam a t tys"
+  "TAbs [a<:tys].t" \<rightleftharpoons> "trm.TAbs a t tys"
+
+subsection {* Typing contexts and Their Domains *}
 
 types ty_context = "(tyvrs\<times>ty) list"
 
-text {* domain of a context --- (the name "dom" is already used elsewhere) *}
 consts
   "domain" :: "ty_context \<Rightarrow> tyvrs set"
 primrec
@@ -49,26 +61,28 @@ lemma finite_domain:
   shows "finite (domain \<Gamma>)"
   by (induct \<Gamma>, auto)
 
-lemma domain_inclusion[rule_format]:
-  shows "(X,T)\<in>set \<Gamma> \<longrightarrow> X\<in>(domain \<Gamma>)"
-  by (induct \<Gamma>, auto)
+lemma domain_inclusion:
+  assumes a: "(X,T)\<in>set \<Gamma>" 
+  shows "X\<in>(domain \<Gamma>)"
+  using a by (induct \<Gamma>, auto)
 
-lemma domain_existence[rule_format]:
-  shows "X\<in>(domain \<Gamma>) \<longrightarrow> (\<exists>T.(X,T)\<in>set \<Gamma>)"
-  by (induct \<Gamma>, auto)
+lemma domain_existence:
+  assumes a: "X\<in>(domain \<Gamma>)" 
+  shows "\<exists>T.(X,T)\<in>set \<Gamma>"
+  using a by (induct \<Gamma>, auto)
 
 lemma domain_append:
   shows "domain (\<Gamma>@\<Delta>) = ((domain \<Gamma>) \<union> (domain \<Delta>))"
   by (induct \<Gamma>, auto)
 
-section {* Two functions over types *}
+section {* Size Functions and Capture Avoiding Substitutiuon for Types *}
 
 text {* they cannot yet be defined conveniently unless we have a recursion combinator *}
 
 consts size_ty :: "ty \<Rightarrow> nat"
 
 lemma size_ty[simp]:
-  shows "size_ty (TyVar X) = 1"
+  shows "size_ty (TVar X) = 1"
   and   "size_ty (Top) = 1"
   and   "\<lbrakk>size_ty t1 = m ; size_ty t2 = n\<rbrakk> \<Longrightarrow> size_ty (t1 \<rightarrow> t2) = m + n + 1"
   and   "\<lbrakk>size_ty t1 = m ; size_ty t2 = n\<rbrakk> \<Longrightarrow> size_ty (\<forall> [a<:t1].t2) = m + n + 1"
@@ -77,7 +91,7 @@ sorry
 consts subst_ty :: "ty \<Rightarrow> tyvrs \<Rightarrow> ty \<Rightarrow> ty"
 
 lemma subst_ty[simp]:
-  shows "subst_ty (TyVar X) Y T = (if X=Y then T else (TyVar X))"
+  shows "subst_ty (TVar X) Y T = (if X=Y then T else (TVar X))"
   and   "subst_ty Top Y T = Top"
   and   "subst_ty (T1 \<rightarrow> T2) Y T = (subst_ty T1 Y T) \<rightarrow> (subst_ty T2 Y T)"
   and   "X\<sharp>(Y,T) \<Longrightarrow> subst_ty (\<forall>[X<:T1].T2) Y T = (\<forall>[X<:(subst_ty T1 Y T)].(subst_ty T2 Y T))"
@@ -90,7 +104,7 @@ primrec
 "subst_ctxt [] Y T = []"
 "subst_ctxt (XT#Xs) Y T = (fst XT, subst_ty (snd XT) Y T)#(subst_ctxt Xs Y T)"
 
-text {* valid contexts *}
+subsection {* valid contexts *}
 
 constdefs
   "closed_in" :: "ty \<Rightarrow> ty_context \<Rightarrow> bool" ("_ closed'_in _" [100,100] 100)
@@ -108,7 +122,7 @@ lemma closed_in_eqvt:
   shows "(pi\<bullet>S) closed_in (pi\<bullet>\<Gamma>)"
   using a
 proof (unfold "closed_in_def")
-  assume "supp S \<subseteq> (domain \<Gamma>)"
+  assume "supp S \<subseteq> (domain \<Gamma>)" 
   hence "pi\<bullet>(supp S) \<subseteq> pi\<bullet>(domain \<Gamma>)"
     by (simp add: pt_subseteq_eqvt[OF pt_tyvrs_inst, OF at_tyvrs_inst])
   thus "(supp (pi\<bullet>S)) \<subseteq> (domain (pi\<bullet>\<Gamma>))"
@@ -142,7 +156,7 @@ next
   proof (simp, rule valid_rel.v2)
     show "\<turnstile> (pi \<bullet> \<Gamma>) ok" using a1 by simp
   next 
-    show "(pi\<bullet>X)\<sharp>(pi\<bullet>\<Gamma>)" using a2 by (simp add: pt_fresh_bij[OF pt_tyvrs_inst, OF at_tyvrs_inst])
+    show "(pi\<bullet>X)\<sharp>(pi\<bullet>\<Gamma>)" using a2 by (simp add: fresh_eqvt)
   next
     show "(pi\<bullet>T) closed_in (pi\<bullet>\<Gamma>)" using a3 by (rule closed_in_eqvt)
   qed
@@ -153,24 +167,20 @@ lemma validE:
   shows "\<turnstile> \<Gamma> ok \<and> X\<sharp>\<Gamma> \<and> T closed_in \<Gamma>"
 using a by (cases, auto)
 
-lemma validE_append[rule_format]:
-  shows "\<turnstile> (\<Delta>@\<Gamma>) ok \<longrightarrow> \<turnstile> \<Gamma> ok"
-  by (induct \<Delta>, auto dest: validE)
+lemma validE_append:
+  assumes a: "\<turnstile> (\<Delta>@\<Gamma>) ok" 
+  shows "\<turnstile> \<Gamma> ok"
+  using a by (induct \<Delta>, auto dest: validE)
 
-lemma domain_fresh[rule_format]:
+lemma domain_fresh:
   fixes X::"tyvrs"
-  shows "\<turnstile> \<Gamma> ok \<longrightarrow> (X\<sharp>(domain \<Gamma>) = X\<sharp>\<Gamma>)"
+  assumes a: "\<turnstile> \<Gamma> ok" 
+  shows "X\<sharp>(domain \<Gamma>) = X\<sharp>\<Gamma>"
+using a
 apply(induct \<Gamma>)
-apply(simp add: fresh_list_nil fresh_set_empty)
-apply(simp add: fresh_list_cons fresh_prod 
-   fresh_fin_insert[OF pt_tyvrs_inst, OF at_tyvrs_inst, OF fs_tyvrs_inst, OF finite_domain])
-apply(rule impI)
-apply(clarify)
-apply(simp add: fresh_prod)
-apply(drule validE)
-apply(simp)
-apply(simp add: closed_in_def2 fresh_def)
-apply(force)
+apply(auto simp add: fresh_list_nil fresh_list_cons fresh_set_empty fresh_prod fresh_atm
+  fresh_fin_insert[OF pt_tyvrs_inst, OF at_tyvrs_inst, OF fs_tyvrs_inst, OF finite_domain])
+apply(force simp add: closed_in_def2 fresh_def)
 done
 
 lemma closed_in_fresh:
@@ -186,8 +196,11 @@ apply(simp add: fresh_def)
 apply(force)
 done
 
-lemma replace_type[rule_format]:
-  shows "\<turnstile> (\<Delta>@(X,T)#\<Gamma>) ok \<longrightarrow> S closed_in \<Gamma> \<longrightarrow> \<turnstile> (\<Delta>@(X,S)#\<Gamma>) ok"
+lemma replace_type:
+  assumes a: "\<turnstile> (\<Delta>@(X,T)#\<Gamma>) ok"
+  and     b: "S closed_in \<Gamma>"
+  shows "\<turnstile> (\<Delta>@(X,S)#\<Gamma>) ok"
+using a b 
 apply(induct \<Delta>)
 apply(auto dest!: validE intro!: v2 simp add: fresh_list_append fresh_list_cons fresh_prod)
 apply(drule validE_append)
@@ -199,9 +212,11 @@ apply(simp add: closed_in_def2)
 apply(simp add: domain_append)
 done
 
-lemma fresh_implies_not_member[rule_format]:
+lemma fresh_implies_not_member:
   fixes \<Gamma>::"ty_context"
-  shows "X\<sharp>\<Gamma> \<longrightarrow> \<not>(\<exists>T.(X,T)\<in>(set \<Gamma>))"
+  assumes a: "X\<sharp>\<Gamma>" 
+  shows "\<not>(\<exists>T.(X,T)\<in>(set \<Gamma>))"
+  using a
   apply (induct \<Gamma>)
   apply (auto dest: validE simp add: fresh_list_cons fresh_prod fresh_atm)
   done
@@ -227,8 +242,8 @@ translations
 inductive subtype_of_rel
 intros
 S_Top[intro]:   "\<lbrakk>\<turnstile> \<Gamma> ok; S closed_in \<Gamma>\<rbrakk> \<Longrightarrow> \<Gamma> \<turnstile> S <: Top"
-S_Var[intro]:   "\<lbrakk>\<turnstile> \<Gamma> ok; (X,S) \<in> (set \<Gamma>); \<Gamma> \<turnstile> S <: T\<rbrakk> \<Longrightarrow> \<Gamma> \<turnstile> (TyVar X) <: T"
-S_Refl[intro]:  "\<lbrakk>\<turnstile> \<Gamma> ok; X \<in> (domain \<Gamma>)\<rbrakk>\<Longrightarrow> \<Gamma> \<turnstile> TyVar X <: TyVar X"
+S_Var[intro]:   "\<lbrakk>\<turnstile> \<Gamma> ok; (X,S) \<in> set \<Gamma>; \<Gamma> \<turnstile> S <: T\<rbrakk> \<Longrightarrow> \<Gamma> \<turnstile> (TVar X) <: T"
+S_Refl[intro]:  "\<lbrakk>\<turnstile> \<Gamma> ok; X \<in> domain \<Gamma>\<rbrakk>\<Longrightarrow> \<Gamma> \<turnstile> TVar X <: TVar X"
 S_Arrow[intro]: "\<lbrakk>\<Gamma> \<turnstile> T1 <: S1; \<Gamma> \<turnstile> S2 <: T2\<rbrakk> \<Longrightarrow> \<Gamma> \<turnstile> (S1 \<rightarrow> S2) <: (T1 \<rightarrow> T2)" 
 S_All[intro]:   "\<lbrakk>\<Gamma> \<turnstile> T1 <: S1; X\<sharp>\<Gamma>; ((X,T1)#\<Gamma>) \<turnstile> S2 <: T2\<rbrakk> 
                   \<Longrightarrow> \<Gamma> \<turnstile> \<forall> [X<:S1].S2 <: \<forall> [X<:T1].T2"  
@@ -239,37 +254,21 @@ lemma subtype_implies_closed:
 using a
 proof (induct)
   case (S_Top S \<Gamma>)
-  have "Top closed_in \<Gamma>" 
-    by (simp add: closed_in_def ty.supp)
+  have "Top closed_in \<Gamma>" by (simp add: closed_in_def ty.supp)
   moreover
   have "S closed_in \<Gamma>" by fact
   ultimately show "S closed_in \<Gamma> \<and> Top closed_in \<Gamma>" by simp
 next
   case (S_Var S T X \<Gamma>)
   have "(X,S)\<in>set \<Gamma>" by fact
-  hence "X\<in>(domain \<Gamma>)" by (rule domain_inclusion)
-  hence "(TyVar X) closed_in \<Gamma>" by (simp add: closed_in_def ty.supp supp_atm)
+  hence "X \<in> domain \<Gamma>" by (rule domain_inclusion)
+  hence "(TVar X) closed_in \<Gamma>" by (simp add: closed_in_def ty.supp supp_atm)
   moreover
   have "S closed_in \<Gamma> \<and> T closed_in \<Gamma>" by fact
   hence "T closed_in \<Gamma>" by force
-  ultimately show "(TyVar X) closed_in \<Gamma> \<and> T closed_in \<Gamma>" by simp
-next
-  case S_Refl thus ?case 
-    by (simp add: closed_in_def ty.supp supp_atm) 
-next
-  case S_Arrow thus ?case by (force simp add: closed_in_def ty.supp)
-next 
-  case S_All thus ?case by (auto simp add: closed_in_def ty.supp abs_supp)
-qed
+  ultimately show "(TVar X) closed_in \<Gamma> \<and> T closed_in \<Gamma>" by simp
+qed (auto simp add: closed_in_def ty.supp supp_atm abs_supp)
 
-text {* a completely automated proof *}
-lemma subtype_implies_closed:
-  assumes a: "\<Gamma> \<turnstile> S <: T"
-  shows "S closed_in \<Gamma> \<and> T closed_in \<Gamma>"
-using a
-apply (induct) 
-apply (auto simp add: closed_in_def ty.supp abs_supp domain_inclusion supp_atm)
-done
 
 lemma subtype_implies_ok:
   fixes X::"tyvrs"
@@ -281,14 +280,15 @@ lemma subtype_implies_fresh:
   fixes X::"tyvrs"
   assumes a1: "\<Gamma> \<turnstile> S <: T"
   and     a2: "X\<sharp>\<Gamma>"
-  shows "X\<sharp>(S,T)"  
+  shows "X\<sharp>S \<and> X\<sharp>T"  
 proof -
   from a1 have "\<turnstile> \<Gamma> ok" by (rule subtype_implies_ok)
-  with a2 have b0: "X\<sharp>domain(\<Gamma>)" by (simp add: domain_fresh)
+  with a2 have "X\<sharp>domain(\<Gamma>)" by (simp add: domain_fresh)
+  moreover
   from a1 have "S closed_in \<Gamma> \<and> T closed_in \<Gamma>" by (rule subtype_implies_closed)
-  hence b1: "supp S \<subseteq> ((supp (domain \<Gamma>))::tyvrs set)" 
-    and b2: "supp T \<subseteq> ((supp (domain \<Gamma>))::tyvrs set)" by (simp_all add: closed_in_def2)
-  thus "X\<sharp>(S,T)" using b0 b1 b2 by (force simp add: supp_prod fresh_def)
+  hence "supp S \<subseteq> ((supp (domain \<Gamma>))::tyvrs set)" 
+    and "supp T \<subseteq> ((supp (domain \<Gamma>))::tyvrs set)" by (simp_all add: closed_in_def2)
+  ultimately show "X\<sharp>S \<and> X\<sharp>T" by (force simp add: supp_prod fresh_def)
 qed
 
 lemma silly_eqvt1:
@@ -322,10 +322,10 @@ done
 lemma subtype_of_rel_induct[consumes 1, case_names S_Top S_Var S_Refl S_Arrow S_All]:
   fixes  P :: "'a::fs_tyvrs\<Rightarrow>ty_context \<Rightarrow> ty \<Rightarrow> ty \<Rightarrow>bool"
   assumes a: "\<Gamma> \<turnstile> S <: T"
-  and a1:    "\<And>\<Gamma> S x. (\<turnstile> \<Gamma> ok) \<Longrightarrow> (S closed_in \<Gamma>) \<Longrightarrow> P x \<Gamma> S Top"
-  and a2:    "\<And>\<Gamma> X S T x. (\<turnstile> \<Gamma> ok) \<Longrightarrow> ((X,S)\<in>set \<Gamma>) \<Longrightarrow> (\<Gamma> \<turnstile> S <: T) \<Longrightarrow> (\<And>z. P z \<Gamma> S T)
-              \<Longrightarrow> P x \<Gamma> (TyVar X) T"
-  and a3:    "\<And>\<Gamma> X x. (\<turnstile> \<Gamma> ok) \<Longrightarrow> X\<in>domain \<Gamma> \<Longrightarrow> P x \<Gamma> (TyVar X) (TyVar X)"  
+  and a1:    "\<And>\<Gamma> S x. \<turnstile> \<Gamma> ok \<Longrightarrow> S closed_in \<Gamma> \<Longrightarrow> P x \<Gamma> S Top"
+  and a2:    "\<And>\<Gamma> X S T x. \<turnstile> \<Gamma> ok \<Longrightarrow> (X,S)\<in>set \<Gamma> \<Longrightarrow> \<Gamma> \<turnstile> S <: T \<Longrightarrow> (\<And>z. P z \<Gamma> S T)
+              \<Longrightarrow> P x \<Gamma> (TVar X) T"
+  and a3:    "\<And>\<Gamma> X x. \<turnstile> \<Gamma> ok \<Longrightarrow> X\<in>domain \<Gamma> \<Longrightarrow> P x \<Gamma> (TVar X) (TVar X)"  
   and a4:    "\<And>\<Gamma> S1 S2 T1 T2 x. \<Gamma> \<turnstile> T1 <: S1 \<Longrightarrow> (\<And>z. P z \<Gamma> T1 S1) \<Longrightarrow> \<Gamma> \<turnstile> S2 <: T2 \<Longrightarrow> 
               (\<And>z. P z \<Gamma> S2 T2) \<Longrightarrow> P x \<Gamma> (S1 \<rightarrow> S2) (T1 \<rightarrow> T2)"
   and a5:    "\<And>\<Gamma> X S1 S2 T1 T2 x. 
@@ -335,13 +335,8 @@ lemma subtype_of_rel_induct[consumes 1, case_names S_Top S_Var S_Refl S_Arrow S_
 proof -
   from a have "\<And>(pi::tyvrs prm) (x::'a::fs_tyvrs). P x (pi\<bullet>\<Gamma>) (pi\<bullet>S) (pi\<bullet>T)"
   proof (induct)
-    case (S_Top S \<Gamma>)
-    have b1: "\<turnstile> \<Gamma> ok" by fact 
-    have b2: "S closed_in \<Gamma>" by fact
-    from b1 have "\<turnstile> (pi\<bullet>\<Gamma>) ok" by (rule valid_eqvt)
-    moreover
-    from b2 have "(pi\<bullet>S) closed_in (pi\<bullet>\<Gamma>)" by (rule closed_in_eqvt)
-    ultimately show "P x (pi \<bullet> \<Gamma>) (pi \<bullet> S) (pi\<bullet>Top)" by (simp add: a1)
+    case (S_Top S \<Gamma>) 
+    thus "P x (pi\<bullet>\<Gamma>) (pi\<bullet>S) (pi\<bullet>Top)" by (force intro: valid_eqvt closed_in_eqvt a1)
   next
     case (S_Var S T X \<Gamma>)
     have b1: "\<turnstile> \<Gamma> ok" by fact 
@@ -357,7 +352,7 @@ proof -
     moreover 
     from b4 have "\<And>x. P x (pi\<bullet>\<Gamma>) (pi\<bullet>S) (pi\<bullet>T)" by simp
     ultimately 
-    show "P x (pi\<bullet>\<Gamma>) (pi\<bullet>(TyVar X)) (pi\<bullet>T)" by (simp add: a2)
+    show "P x (pi\<bullet>\<Gamma>) (pi\<bullet>(TVar X)) (pi\<bullet>T)" by (simp add: a2)
   next
     case (S_Refl X \<Gamma>)
     have b1: "\<turnstile> \<Gamma> ok" by fact
@@ -366,9 +361,9 @@ proof -
     moreover
     from b2 have "(pi\<bullet>X)\<in>pi\<bullet>domain \<Gamma>" by (rule pt_set_bij2[OF pt_tyvrs_inst, OF at_tyvrs_inst])
     hence "(pi\<bullet>X)\<in>domain (pi\<bullet>\<Gamma>)" by (simp add: domain_eqvt pt_list_set_pi[OF pt_tyvrs_inst])
-    ultimately show "P x (pi\<bullet>\<Gamma>) (pi\<bullet>(TyVar X)) (pi\<bullet>(TyVar X))" by (simp add: a3)
+    ultimately show "P x (pi\<bullet>\<Gamma>) (pi\<bullet>(TVar X)) (pi\<bullet>(TVar X))" by (simp add: a3)
   next
-    case S_Arrow thus ?case by (simp, auto intro!: a4 subtype_eqvt)
+    case S_Arrow thus ?case by (auto intro: a4 subtype_eqvt)
   next
     case (S_All S1 S2 T1 T2 X \<Gamma>)
     have b1: "\<Gamma> \<turnstile> T1 <: S1" by fact 
@@ -376,7 +371,7 @@ proof -
     have b4: "((X,T1)#\<Gamma>) \<turnstile> S2 <: T2" by fact
     have b5: "\<And>(pi::tyvrs prm) x. P x (pi\<bullet>((X,T1)#\<Gamma>)) (pi\<bullet>S2) (pi\<bullet>T2)" by fact
     have b3': "X\<sharp>\<Gamma>" by fact
-    have b3'': "X\<sharp>(T1,S1)" using b1 b3' by (rule subtype_implies_fresh)
+    have b3'': "X\<sharp>T1" "X\<sharp>S1" using b1 b3' by (simp_all add: subtype_implies_fresh)
     have b3: "X\<sharp>(\<Gamma>,S1,T1)" using b3' b3'' by (simp add: fresh_prod)
     have "\<exists>C::tyvrs. C\<sharp>(pi\<bullet>X,pi\<bullet>S2,pi\<bullet>T2,pi\<bullet>S1,pi\<bullet>T1,pi\<bullet>\<Gamma>,x)"
       by (rule at_exists_fresh[OF at_tyvrs_inst], simp add: fs_tyvrs1)
@@ -423,27 +418,28 @@ proof -
   thus ?thesis by simp
 qed
 
-section {* Two proofs for reflexivity of subtyping *}
+subsection {* Reflexivity of Subtyping *}
 
 lemma subtype_reflexivity:
   assumes a: "\<turnstile> \<Gamma> ok"
-  and     b: "T closed_in \<Gamma>"
+  and b: "T closed_in \<Gamma>"
   shows "\<Gamma> \<turnstile> T <: T"
 using a b
 proof(nominal_induct T avoiding: \<Gamma> rule: ty.induct_unsafe)
-  case (TAll X T1 T2)
-  have i1: "\<And>\<Gamma>. \<turnstile> \<Gamma> ok \<Longrightarrow> T1 closed_in \<Gamma> \<Longrightarrow> \<Gamma> \<turnstile> T1 <: T1" by fact 
-  have i2: "\<And>\<Gamma>. \<turnstile> \<Gamma> ok \<Longrightarrow> T2 closed_in \<Gamma> \<Longrightarrow> \<Gamma> \<turnstile> T2 <: T2" by fact
-  have f: "X\<sharp>\<Gamma>" by fact
-  have "(\<forall>[X<:T2].T1) closed_in \<Gamma>" by fact
-  hence b1: "T2 closed_in \<Gamma>" and b2: "T1 closed_in ((X,T2)#\<Gamma>)" 
-      by (auto simp add: closed_in_def ty.supp abs_supp)
-  have c1: "\<turnstile> \<Gamma> ok" by fact  
-  hence c2: "\<turnstile> ((X,T2)#\<Gamma>) ok" using b1 f by force
-  have "\<Gamma> \<turnstile> T2 <: T2" using i2 b1 c1 by simp
+  case (TAll X T\<^isub>1 T\<^isub>2)
+  have ih_T\<^isub>1: "\<And>\<Gamma>. \<turnstile> \<Gamma> ok \<Longrightarrow> T\<^isub>1 closed_in \<Gamma> \<Longrightarrow> \<Gamma> \<turnstile> T\<^isub>1 <: T\<^isub>1" by fact 
+  have ih_T\<^isub>2: "\<And>\<Gamma>. \<turnstile> \<Gamma> ok \<Longrightarrow> T\<^isub>2 closed_in \<Gamma> \<Longrightarrow> \<Gamma> \<turnstile> T\<^isub>2 <: T\<^isub>2" by fact
+  have fresh_cond: "X\<sharp>\<Gamma>" by fact
+  have "(\<forall>[X<:T\<^isub>2].T\<^isub>1) closed_in \<Gamma>" by fact
+  hence closed\<^isub>T\<^isub>2: "T\<^isub>2 closed_in \<Gamma>" and closed\<^isub>T\<^isub>1: "T\<^isub>1 closed_in ((X,T\<^isub>2)#\<Gamma>)" 
+    by (auto simp add: closed_in_def ty.supp abs_supp)
+  have ok: "\<turnstile> \<Gamma> ok" by fact  
+  hence ok': "\<turnstile> ((X,T\<^isub>2)#\<Gamma>) ok" using closed\<^isub>T\<^isub>2 fresh_cond by force
+  have "\<Gamma> \<turnstile> T\<^isub>2 <: T\<^isub>2" using ih_T\<^isub>2 closed\<^isub>T\<^isub>2 ok by simp
   moreover
-  have "((X,T2)#\<Gamma>) \<turnstile> T1 <: T1" using i1 b2 c2 by simp
-  ultimately show "\<Gamma> \<turnstile> \<forall>[X<:T2].T1 <: \<forall>[X<:T2].T1" using f by force
+  have "((X,T\<^isub>2)#\<Gamma>) \<turnstile> T\<^isub>1 <: T\<^isub>1" using ih_T\<^isub>1 closed\<^isub>T\<^isub>1 ok' by simp
+  ultimately show "\<Gamma> \<turnstile> \<forall>[X<:T\<^isub>2].T\<^isub>1 <: \<forall>[X<:T\<^isub>2].T\<^isub>1" using fresh_cond 
+    by (simp add: subtype_of_rel.S_All)
 qed (auto simp add: closed_in_def ty.supp supp_atm)
 
 lemma subtype_reflexivity:
@@ -453,24 +449,24 @@ lemma subtype_reflexivity:
 using a b
 apply(nominal_induct T avoiding: \<Gamma> rule: ty.induct_unsafe)
 apply(auto simp add: ty.supp abs_supp closed_in_def supp_atm)
-(* too bad that this cannot be found automatically *)
+--{* Too bad that this instantiation cannot be found automatically. *}
 apply(drule_tac x="(tyvrs, ty2)#\<Gamma>" in meta_spec)
 apply(force simp add: closed_in_def)
 done
 
-text {* Inversion lemmas. . .  *}
+text {* Inversion lemmas *}
 lemma S_TopE:
- shows "\<Gamma> \<turnstile> Top <: T \<Longrightarrow> T = Top" 
-apply(ind_cases "\<Gamma> \<turnstile> Top <: T", auto)
-done
+  assumes a: "\<Gamma> \<turnstile> Top <: T"
+  shows "T = Top"
+using a by (cases, auto) 
 
 lemma S_ArrowE_left:
   assumes a: "\<Gamma> \<turnstile> S1 \<rightarrow> S2 <: T" 
   shows "T = Top \<or> (\<exists>T1 T2. T = T1 \<rightarrow> T2 \<and> \<Gamma> \<turnstile> T1 <: S1 \<and> \<Gamma> \<turnstile> S2 <: T2)"
-using  a by (cases, auto simp add: ty.inject)
+using a by (cases, auto simp add: ty.inject)
 
 lemma S_AllE_left:
-  shows "\<lbrakk>\<Gamma> \<turnstile> \<forall>[X<:S1].S2 <: T; X\<sharp>(\<Gamma>,S1)\<rbrakk>
+  shows "\<lbrakk>\<Gamma> \<turnstile> \<forall>[X<:S1].S2 <: T; X\<sharp>\<Gamma>; X\<sharp>S1\<rbrakk>
          \<Longrightarrow> T = Top \<or> (\<exists>T1 T2. T = \<forall>[X<:T1].T2 \<and> \<Gamma> \<turnstile> T1 <: S1 \<and> ((X,T1)#\<Gamma>) \<turnstile> S2 <: T2)"
   apply(frule subtype_implies_ok)
   apply(ind_cases "\<Gamma> \<turnstile> \<forall>[X<:S1].S2 <: T")
@@ -486,10 +482,9 @@ lemma S_AllE_left:
   (* 1st conjunct *)
   apply(rule conjI)
   apply(simp add: pt_fresh_left[OF pt_tyvrs_inst, OF at_tyvrs_inst] calc_atm)
-  apply(simp add: fresh_prod)
   apply(drule_tac \<Gamma>="((Xa,T1)#\<Gamma>)" in  subtype_implies_closed)+
   apply(simp add: closed_in_def)
-  apply(auto simp add: domain_fresh[of "\<Gamma>" "X", symmetric])
+  apply(simp add: domain_fresh[of "\<Gamma>" "X", symmetric])
   apply(simp add: fresh_def)
   apply(subgoal_tac "X \<notin> (insert Xa (domain \<Gamma>))")(*A*)
   apply(force)
@@ -497,7 +492,7 @@ lemma S_AllE_left:
   apply(simp add: at_fin_set_supp[OF at_tyvrs_inst, OF finite_domain])
   (* 2nd conjunct *)
   apply(frule_tac X="X" in subtype_implies_fresh)
-  apply(simp add: fresh_prod)
+  apply(assumption)
   apply(drule_tac X="Xa" in subtype_implies_fresh)
   apply(assumption)
   apply(simp add: fresh_prod)
@@ -506,19 +501,22 @@ lemma S_AllE_left:
   apply(simp add: pt_fresh_fresh[OF pt_tyvrs_inst, OF at_tyvrs_inst])
   done
 
-section {* Type substitution *}
+section {* Type Substitution *}
 
-lemma subst_ty_fresh[rule_format]:
-  fixes P :: "ty"
-  and   X :: "tyvrs"
-  shows "X\<sharp>(T,P) \<longrightarrow> X\<sharp>(subst_ty T Y P)"
+lemma subst_ty_fresh:
+  fixes X :: "tyvrs"
+  assumes a: "X\<sharp>(T,P)"
+  shows "X\<sharp>(subst_ty T Y P)"
+  using a
   apply (nominal_induct T avoiding : T Y P rule: ty.induct_unsafe)
   apply (auto simp add: fresh_prod abs_fresh)
   done
 
-lemma subst_ctxt_fresh[rule_format]:
+lemma subst_ctxt_fresh:
   fixes X::"tyvrs"
-  shows "X\<sharp>(\<Gamma>,P) \<longrightarrow> X\<sharp>(subst_ctxt \<Gamma> Y P)"
+  assumes a: "X\<sharp>(\<Gamma>,P)"
+  shows "X\<sharp>(subst_ctxt \<Gamma> Y P)"
+  using a
   apply (induct \<Gamma>)
   apply (auto intro: subst_ty_fresh simp add: fresh_prod fresh_list_cons)
   done
@@ -596,10 +594,16 @@ lemma extends_closed:
   using a1 a2
   by (auto dest: extends_domain simp add: closed_in_def)
 
+lemma extends_memb:
+  assumes a: "\<Delta> extends \<Gamma>"
+  and b: "(X,T) \<in> set \<Gamma>"
+  shows "(X,T) \<in> set \<Delta>"
+  using a b by (simp add: extends_def)
+
 lemma weakening:
   assumes a: "\<Gamma> \<turnstile> S <: T"
-  and     b: "\<turnstile> \<Delta> ok"
-  and     c: "\<Delta> extends \<Gamma>"
+  and b: "\<turnstile> \<Delta> ok"
+  and c: "\<Delta> extends \<Gamma>"
   shows "\<Delta> \<turnstile> S <: T"
   using a b c 
 proof (nominal_induct \<Gamma> S T avoiding: \<Delta> rule: subtype_of_rel_induct)
@@ -608,7 +612,7 @@ proof (nominal_induct \<Gamma> S T avoiding: \<Delta> rule: subtype_of_rel_induc
   have "\<turnstile> \<Delta> ok" by fact
   moreover
   have "\<Delta> extends \<Gamma>" by fact
-  hence "S closed_in \<Delta>" using lh_drv_prem by (rule_tac extends_closed)
+  hence "S closed_in \<Delta>" using lh_drv_prem by (simp only: extends_closed)
   ultimately show "\<Delta> \<turnstile> S <: Top" by force
 next 
   case (S_Var \<Gamma> X S T)
@@ -616,10 +620,10 @@ next
   have ih: "\<And>\<Delta>. \<turnstile> \<Delta> ok \<Longrightarrow> \<Delta> extends \<Gamma> \<Longrightarrow> \<Delta> \<turnstile> S <: T" by fact
   have ok: "\<turnstile> \<Delta> ok" by fact
   have extends: "\<Delta> extends \<Gamma>" by fact
-  have "(X,S) \<in> set \<Delta>" using lh_drv_prem extends by (simp add: extends_def)
+  have "(X,S) \<in> set \<Delta>" using lh_drv_prem extends by (simp only: extends_memb)
   moreover
   have "\<Delta> \<turnstile> S <: T" using ok extends ih by simp
-  ultimately show "\<Delta> \<turnstile> TyVar X <: T" using ok by force
+  ultimately show "\<Delta> \<turnstile> TVar X <: T" using ok by force
 next
   case (S_Refl \<Gamma> X)
   have lh_drv_prem: "X \<in> domain \<Gamma>" by fact
@@ -627,90 +631,84 @@ next
   moreover
   have "\<Delta> extends \<Gamma>" by fact
   hence "X \<in> domain \<Delta>" using lh_drv_prem by (force dest: extends_domain)
-  ultimately show "\<Delta> \<turnstile> TyVar X <: TyVar X" by force
+  ultimately show "\<Delta> \<turnstile> TVar X <: TVar X" by force
 next 
-  case S_Arrow thus ?case by force
+  case (S_Arrow \<Gamma> S\<^isub>1 S\<^isub>2 T\<^isub>1 T\<^isub>2) thus "\<Delta> \<turnstile> S\<^isub>1 \<rightarrow> S\<^isub>2 <: T\<^isub>1 \<rightarrow> T\<^isub>2" by blast
 next
-  case (S_All \<Gamma> X S1 S2 T1 T2)
-  have fresh: "X\<sharp>\<Delta>" by fact
-  have ih1: "\<And>\<Delta>. \<turnstile> \<Delta> ok \<Longrightarrow> \<Delta> extends \<Gamma> \<Longrightarrow> \<Delta> \<turnstile> T1 <: S1" by fact
-  have ih2: "\<And>\<Delta>. \<turnstile> \<Delta> ok \<Longrightarrow> \<Delta> extends ((X,T1)#\<Gamma>) \<Longrightarrow> \<Delta> \<turnstile> S2 <: T2" by fact
-  have lh_drv_prem: "\<Gamma> \<turnstile> T1 <: S1" by fact
-  hence b5: "T1 closed_in \<Gamma>" by (simp add: subtype_implies_closed) 
+  case (S_All \<Gamma> X S\<^isub>1 S\<^isub>2 T\<^isub>1 T\<^isub>2)
+  have fresh_cond: "X\<sharp>\<Delta>" by fact
+  have ih\<^isub>1: "\<And>\<Delta>. \<turnstile> \<Delta> ok \<Longrightarrow> \<Delta> extends \<Gamma> \<Longrightarrow> \<Delta> \<turnstile> T\<^isub>1 <: S\<^isub>1" by fact
+  have ih\<^isub>2: "\<And>\<Delta>. \<turnstile> \<Delta> ok \<Longrightarrow> \<Delta> extends ((X,T\<^isub>1)#\<Gamma>) \<Longrightarrow> \<Delta> \<turnstile> S\<^isub>2 <: T\<^isub>2" by fact
+  have lh_drv_prem: "\<Gamma> \<turnstile> T\<^isub>1 <: S\<^isub>1" by fact
+  hence closed\<^isub>T\<^isub>1: "T\<^isub>1 closed_in \<Gamma>" by (simp add: subtype_implies_closed) 
   have ok: "\<turnstile> \<Delta> ok" by fact
-  have extends: "\<Delta> extends \<Gamma>" by fact
-  have "T1 closed_in \<Delta>" using extends b5 by (simp only: extends_closed)
-  hence "\<turnstile> ((X,T1)#\<Delta>) ok" using fresh ok by force   
+  have ext: "\<Delta> extends \<Gamma>" by fact
+  have "T\<^isub>1 closed_in \<Delta>" using ext closed\<^isub>T\<^isub>1 by (simp only: extends_closed)
+  hence "\<turnstile> ((X,T\<^isub>1)#\<Delta>) ok" using fresh_cond ok by force   
   moreover 
-  have "((X,T1)#\<Delta>) extends ((X,T1)#\<Gamma>)" using extends by (force simp add: extends_def)
-  ultimately have "((X,T1)#\<Delta>) \<turnstile> S2 <: T2" using ih2 by simp
+  have "((X,T\<^isub>1)#\<Delta>) extends ((X,T\<^isub>1)#\<Gamma>)" using ext by (force simp add: extends_def)
+  ultimately have "((X,T\<^isub>1)#\<Delta>) \<turnstile> S\<^isub>2 <: T\<^isub>2" using ih\<^isub>2 by simp
   moreover
-  have "\<Delta> \<turnstile> T1 <: S1" using ok extends ih1 by simp 
-  ultimately show "\<Delta> \<turnstile> \<forall> [X<:S1].S2 <: \<forall> [X<:T1].T2" using ok by (force intro: S_All) 
+  have "\<Delta> \<turnstile> T\<^isub>1 <: S\<^isub>1" using ok ext ih\<^isub>1 by simp 
+  ultimately show "\<Delta> \<turnstile> \<forall> [X<:S\<^isub>1].S\<^isub>2 <: \<forall> [X<:T\<^isub>1].T\<^isub>2" using ok by (force intro: S_All)
 qed
 
-text {* more automated proof *}
+text {* In fact all "non-binding" cases can be solved automatically: *}
 
 lemma weakening:
   assumes a: "\<Gamma> \<turnstile> S <: T"
-  and     b: "\<turnstile> \<Delta> ok"
-  and     c: "\<Delta> extends \<Gamma>"
+  and b: "\<turnstile> \<Delta> ok"
+  and c: "\<Delta> extends \<Gamma>"
   shows "\<Delta> \<turnstile> S <: T"
   using a b c 
 proof (nominal_induct \<Gamma> S T avoiding: \<Delta> rule: subtype_of_rel_induct)
-  case (S_Top \<Gamma> S) thus ?case by (force intro: extends_closed)
-next 
-  case (S_Var \<Gamma> X S T) thus ?case by (force simp add: extends_def)
-next
-  case (S_Refl \<Gamma> X) thus ?case by (force dest: extends_domain)
-next 
-  case S_Arrow thus ?case by force
-next
-  case (S_All \<Gamma> X S1 S2 T1 T2)
-  have fresh: "X\<sharp>\<Delta>" by fact
-  have ih1: "\<And>\<Delta>. \<turnstile> \<Delta> ok \<Longrightarrow> \<Delta> extends \<Gamma> \<Longrightarrow> \<Delta> \<turnstile> T1 <: S1" by fact
-  have ih2: "\<And>\<Delta>. \<turnstile> \<Delta> ok \<Longrightarrow> \<Delta> extends ((X,T1)#\<Gamma>) \<Longrightarrow> \<Delta> \<turnstile> S2 <: T2" by fact
-  have lh_drv_prem: "\<Gamma> \<turnstile> T1 <: S1" by fact
-  hence b5: "T1 closed_in \<Gamma>" by (simp add: subtype_implies_closed) 
+  case (S_All \<Gamma> X S\<^isub>1 S\<^isub>2 T\<^isub>1 T\<^isub>2)
+  have fresh_cond: "X\<sharp>\<Delta>" by fact
+  have ih\<^isub>1: "\<And>\<Delta>. \<turnstile> \<Delta> ok \<Longrightarrow> \<Delta> extends \<Gamma> \<Longrightarrow> \<Delta> \<turnstile> T\<^isub>1 <: S\<^isub>1" by fact
+  have ih\<^isub>2: "\<And>\<Delta>. \<turnstile> \<Delta> ok \<Longrightarrow> \<Delta> extends ((X,T\<^isub>1)#\<Gamma>) \<Longrightarrow> \<Delta> \<turnstile> S\<^isub>2 <: T\<^isub>2" by fact
+  have lh_drv_prem: "\<Gamma> \<turnstile> T\<^isub>1 <: S\<^isub>1" by fact
+  hence closed\<^isub>T\<^isub>1: "T\<^isub>1 closed_in \<Gamma>" by (simp add: subtype_implies_closed) 
   have ok: "\<turnstile> \<Delta> ok" by fact
-  have extends: "\<Delta> extends \<Gamma>" by fact
-  have "T1 closed_in \<Delta>" using extends b5 by (simp only: extends_closed)
-  hence "\<turnstile> ((X,T1)#\<Delta>) ok" using fresh ok by force   
+  have ext: "\<Delta> extends \<Gamma>" by fact
+  have "T\<^isub>1 closed_in \<Delta>" using ext closed\<^isub>T\<^isub>1 by (simp only: extends_closed)
+  hence "\<turnstile> ((X,T\<^isub>1)#\<Delta>) ok" using fresh_cond ok by force   
   moreover 
-  have "((X,T1)#\<Delta>) extends ((X,T1)#\<Gamma>)" using extends by (force simp add: extends_def)
-  ultimately have "((X,T1)#\<Delta>) \<turnstile> S2 <: T2" using ih2 by simp
+  have "((X,T\<^isub>1)#\<Delta>) extends ((X,T\<^isub>1)#\<Gamma>)" using ext by (force simp add: extends_def)
+  ultimately have "((X,T\<^isub>1)#\<Delta>) \<turnstile> S\<^isub>2 <: T\<^isub>2" using ih\<^isub>2 by simp
   moreover
-  have "\<Delta> \<turnstile> T1 <: S1" using ok extends ih1 by simp 
-  ultimately show "\<Delta> \<turnstile> \<forall> [X<:S1].S2 <: \<forall> [X<:T1].T2" using ok by (force intro: S_All) 
-qed
+  have "\<Delta> \<turnstile> T\<^isub>1 <: S\<^isub>1" using ok ext ih\<^isub>1 by simp 
+  ultimately show "\<Delta> \<turnstile> \<forall> [X<:S\<^isub>1].S\<^isub>2 <: \<forall> [X<:T\<^isub>1].T\<^isub>2" using ok by (force intro: S_All)
+qed (blast intro: extends_closed extends_memb dest: extends_domain)+
 
+text {* our contexts grow from right to left *}
 
 lemma transitivity_and_narrowing:
   shows "\<Gamma> \<turnstile> S <: Q \<Longrightarrow> \<Gamma> \<turnstile> Q <: T \<Longrightarrow> \<Gamma> \<turnstile> S <: T"
-  and   "(\<Delta>@(X,Q)#\<Gamma>) \<turnstile> M <: N \<Longrightarrow> \<Gamma> \<turnstile> P <: Q \<Longrightarrow> (\<Delta>@(X,P)#\<Gamma>) \<turnstile> M <: N"
+  and "(\<Delta>@[(X,Q)]@\<Gamma>) \<turnstile> M <: N \<Longrightarrow> \<Gamma> \<turnstile> P <: Q \<Longrightarrow> (\<Delta>@[(X,P)]@\<Gamma>) \<turnstile> M <: N"
 proof (induct Q fixing: \<Gamma> S T and \<Delta> \<Gamma> X P M N taking: "size_ty" rule: measure_induct_rule)
-  case (less Q)
-  note  IH1_outer = less[THEN conjunct1, rule_format]
-    and IH2_outer = less[THEN conjunct2, THEN spec, of _ "[]", simplified, rule_format]
+  case (less Q) 
+  note IH_trans = prems[THEN conjunct1, rule_format]
+  note IH_narrow = prems[THEN conjunct2, THEN spec, of _ "[]", simplified, rule_format]
 
+    --{* The inner induction for transitivity over @{term "\<Gamma> \<turnstile> S <: Q"} *}
   have transitivity: 
     "\<And>\<Gamma> S T. \<Gamma> \<turnstile> S <: Q \<Longrightarrow> \<Gamma> \<turnstile> Q <: T \<Longrightarrow> \<Gamma> \<turnstile> S <: T"
   proof - 
     
-  -- {* We first handle the case where T = Top once and for all; this saves some 
-        repeated argument below (just like on paper :-).  We establish a little lemma
-        that is invoked where needed in each case of the induction. *} 
+      -- {* We first handle the case where T = Top once and for all; this saves some 
+      repeated argument below (just like on paper :-).  To do so we establish a little 
+      lemma that is invoked where needed in the induction for transitivity. *} 
     have top_case: 
       "\<And>\<Gamma> S T' P. \<lbrakk>\<turnstile> \<Gamma> ok; S closed_in \<Gamma>; P \<Longrightarrow> \<Gamma> \<turnstile> S <: T'; T'=Top \<or> P\<rbrakk> \<Longrightarrow> \<Gamma> \<turnstile> S <: T'"
     proof - 
       fix \<Gamma> S T' P
-      assume S_Top_prem1: "S closed_in \<Gamma>"
-	and  S_Top_prem2: "\<turnstile> \<Gamma> ok"
+      assume S_Top_prm1: "S closed_in \<Gamma>"
+	and  S_Top_prm2: "\<turnstile> \<Gamma> ok"
 	and  alternative: "P \<Longrightarrow> \<Gamma> \<turnstile> S <: T'" 
 	and  "T'=Top \<or> P" 
       moreover
       { assume "T'=Top"
-	hence "\<Gamma> \<turnstile> S <: T'" using S_Top_prem1 S_Top_prem2 by (simp add: S_Top)
+	hence "\<Gamma> \<turnstile> S <: T'" using S_Top_prm1 S_Top_prm2 by (simp add: S_Top)
       } 
       moreover 
       { assume P 
@@ -719,199 +717,184 @@ proof (induct Q fixing: \<Gamma> S T and \<Delta> \<Gamma> X P M N taking: "size
       ultimately show "\<Gamma> \<turnstile> S <: T'" by blast
     qed
 
-    (* Now proceed by induction on the left-hand derivation *)
-    fix \<Gamma> S T
-    assume a: "\<Gamma> \<turnstile> S <: Q" 
-    assume b: "\<Gamma> \<turnstile> Q <: T"
-    from a b show "\<Gamma> \<turnstile> S <: T"
-    proof(nominal_induct \<Gamma> S Q\<equiv>Q avoiding: \<Gamma> S T rule: subtype_of_rel_induct)
-      case (S_Top \<Gamma>1 S1) --{* lh drv.: @{term "\<Gamma> \<turnstile> S <: Q \<equiv> \<Gamma>1 \<turnstile> S1 <: Top"} *}
-      have lh_drv_prem1: "\<turnstile> \<Gamma>1 ok" by fact
-      have lh_drv_prem2: "S1 closed_in \<Gamma>1" by fact
-      have Q_inst: "Top=Q" by fact
-      have rh_drv: "\<Gamma>1 \<turnstile> Q <: T" --"rh drv." by fact
-      hence "T = Top" using Q_inst by (simp add: S_TopE)
-      thus "\<Gamma>1 \<turnstile> S1 <: T" using top_case[of "\<Gamma>1" "S1" "False" "T"] lh_drv_prem1 lh_drv_prem2 by blast
+	--{* Now proceed by the inner induction on the left-hand derivation *}
+    fix \<Gamma>' S' T
+    assume a: "\<Gamma>' \<turnstile> S' <: Q" --{* lh derivation *}
+    assume b: "\<Gamma>' \<turnstile> Q <: T" --{* rh derivation *}
+    from a b show "\<Gamma>' \<turnstile> S' <: T"
+    proof(nominal_induct \<Gamma>' S' Q\<equiv>Q avoiding: \<Gamma>' S' T rule: subtype_of_rel_induct)
+      case (S_Top \<Gamma> S) 
+	--{* in this case lh drv is @{term "\<Gamma> \<turnstile> S <: Top"} *}
+      hence rh_drv: "\<Gamma> \<turnstile> Top <: T" by simp
+      hence T_inst: "T = Top" by (simp add: S_TopE)
+      have lh_drv_prm1: "\<turnstile> \<Gamma> ok" by fact
+      have lh_drv_prm2: "S closed_in \<Gamma>" by fact
+      from lh_drv_prm1 lh_drv_prm2 have "\<Gamma> \<turnstile> S <: Top" by (simp add: subtype_of_rel.S_Top)
+      thus "\<Gamma> \<turnstile> S <: T" using T_inst by simp
     next
-      case (S_Var \<Gamma>1 X1 S1 T1) --{* lh drv.: @{term "\<Gamma> \<turnstile> S <: Q \<equiv> \<Gamma>1 \<turnstile> TVar(X1) <: S1"} *}
-      have lh_drv_prem1: "\<turnstile> \<Gamma>1 ok" by fact
-      have lh_drv_prem2: "(X1,S1)\<in>set \<Gamma>1" by fact
-      have IH_inner: "\<And>T. \<Gamma>1 \<turnstile> Q <: T \<Longrightarrow> T1=Q \<Longrightarrow> \<Gamma>1 \<turnstile> S1 <: T" by fact
-      have Q_inst: "T1=Q" by fact
-      have rh_drv: "\<Gamma>1 \<turnstile> Q <: T" by fact 
-      with IH_inner have "\<Gamma>1 \<turnstile> S1 <: T" using Q_inst by simp
-      thus "\<Gamma>1 \<turnstile> TyVar X1 <: T" using lh_drv_prem1 lh_drv_prem2 by (simp add: subtype_of_rel.S_Var)
+      case (S_Var \<Gamma> Y U Q) 
+	--{* in this case lh drv is @{term "\<Gamma> \<turnstile> TVar(Y) <: Q"} *}
+      hence IH_inner: "\<Gamma> \<turnstile> U <: T" by simp
+      have lh_drv_prm1: "\<turnstile> \<Gamma> ok" by fact
+      have lh_drv_prm2: "(Y,U)\<in>set \<Gamma>" by fact
+      from IH_inner show "\<Gamma> \<turnstile> TVar Y <: T" using lh_drv_prm1 lh_drv_prm2 
+	by (simp add: subtype_of_rel.S_Var)
     next
-      case S_Refl --{* @{text S_Refl} case *} 
-	thus ?case by simp
+      case (S_Refl \<Gamma> X) 
+	--{* in this case lh drv is @{term "\<Gamma> \<turnstile> TVar X <: TVar X"} *}
+      thus "\<Gamma> \<turnstile> TVar X <: T" by simp
     next
-      case (S_Arrow \<Gamma>1 S1 S2 T1 T2) --{* lh drv.: @{term "\<Gamma> \<turnstile> S <: Q \<equiv> \<Gamma>1 \<turnstile> S1 \<rightarrow> S2 <: T1 \<rightarrow> T2"} *}
-      have lh_drv_prem1: "\<Gamma>1 \<turnstile> T1 <: S1" by fact
-      have lh_drv_prem2: "\<Gamma>1 \<turnstile> S2 <: T2" by fact
-      have rh_deriv: "\<Gamma>1 \<turnstile> Q <: T" by fact
-      have Q_inst: "T1 \<rightarrow> T2 = Q" by fact
-      have measure: "size_ty T1 < size_ty Q" "size_ty T2 < size_ty Q " using Q_inst by force+
-      have "S1 closed_in \<Gamma>1" and "S2 closed_in \<Gamma>1" 
-	using lh_drv_prem1 lh_drv_prem2 by (simp_all add: subtype_implies_closed)
-      hence "(S1 \<rightarrow> S2) closed_in \<Gamma>1" by (simp add: closed_in_def ty.supp)
+      case (S_Arrow \<Gamma> S1 S2 Q1 Q2) 
+	--{* in this case lh drv is @{term "\<Gamma> \<turnstile> S1 \<rightarrow> S2 <: Q1 \<rightarrow> Q2"} *}
+      hence rh_drv: "\<Gamma> \<turnstile> Q1 \<rightarrow> Q2 <: T" by simp
+      have Q_inst: "Q1 \<rightarrow> Q2 = Q" by fact
+      hence Q1_less: "size_ty Q1 < size_ty Q" 
+	and Q2_less: "size_ty Q2 < size_ty Q" by auto
+      have lh_drv_prm1: "\<Gamma> \<turnstile> Q1 <: S1" by fact
+      have lh_drv_prm2: "\<Gamma> \<turnstile> S2 <: Q2" by fact      
+      have "S1 closed_in \<Gamma>" and "S2 closed_in \<Gamma>" 
+	using lh_drv_prm1 lh_drv_prm2 by (simp_all add: subtype_implies_closed)
+      hence "(S1 \<rightarrow> S2) closed_in \<Gamma>" by (simp add: closed_in_def ty.supp)
       moreover
-      have "\<turnstile> \<Gamma>1 ok" using rh_deriv by (rule subtype_implies_ok)
+      have "\<turnstile> \<Gamma> ok" using rh_drv by (rule subtype_implies_ok)
       moreover
-      have "T = Top \<or> (\<exists>T3 T4.  T= T3 \<rightarrow> T4 \<and> \<Gamma>1 \<turnstile> T3 <: T1 \<and> \<Gamma>1 \<turnstile> T2 <: T4)" 
-	using rh_deriv Q_inst by (simp add:S_ArrowE_left)  
+      from rh_drv have "T = Top \<or> (\<exists>T1 T2.  T = T1 \<rightarrow> T2 \<and> \<Gamma> \<turnstile> T1 <: Q1 \<and> \<Gamma> \<turnstile> Q2 <: T2)" 
+	by (simp add: S_ArrowE_left)  
       moreover
-      { assume "\<exists>T3 T4. T= T3 \<rightarrow> T4 \<and> \<Gamma>1 \<turnstile> T3 <: T1 \<and> \<Gamma>1 \<turnstile> T2 <: T4"
-	then obtain T3 T4 
-	  where T_inst: "T= T3 \<rightarrow> T4" 
-	  and   rh_drv_prem1: "\<Gamma>1 \<turnstile> T3 <: T1"
-	  and   rh_drv_prem2: "\<Gamma>1 \<turnstile> T2 <: T4" by force
-        from IH1_outer[of "T1"] have "\<Gamma>1 \<turnstile> T3 <: S1" using measure rh_drv_prem1 lh_drv_prem1 by blast
+      { assume "\<exists>T1 T2. T = T1 \<rightarrow> T2 \<and> \<Gamma> \<turnstile> T1 <: Q1 \<and> \<Gamma> \<turnstile> Q2 <: T2"
+	then obtain T1 T2 
+	  where T_inst: "T = T1 \<rightarrow> T2" 
+	  and   rh_drv_prm1: "\<Gamma> \<turnstile> T1 <: Q1"
+	  and   rh_drv_prm2: "\<Gamma> \<turnstile> Q2 <: T2" by force
+        from IH_trans[of "Q1"] have "\<Gamma> \<turnstile> T1 <: S1" using Q1_less rh_drv_prm1 lh_drv_prm1 by simp 
 	moreover
-	from IH1_outer[of "T2"] have "\<Gamma>1 \<turnstile> S2 <: T4" using measure rh_drv_prem2 lh_drv_prem2 by blast
-	ultimately have "\<Gamma>1 \<turnstile> S1 \<rightarrow> S2 <: T" using T_inst by force
+	from IH_trans[of "Q2"] have "\<Gamma> \<turnstile> S2 <: T2" using Q2_less rh_drv_prm2 lh_drv_prm2 by simp
+	ultimately have "\<Gamma> \<turnstile> S1 \<rightarrow> S2 <: T1 \<rightarrow> T2" by (simp add: subtype_of_rel.S_Arrow)
+	hence "\<Gamma> \<turnstile> S1 \<rightarrow> S2 <: T" using T_inst by simp
       }
-      ultimately show "\<Gamma>1 \<turnstile> S1 \<rightarrow> S2 <: T" using top_case[of "\<Gamma>1" "S1\<rightarrow>S2" _ "T'"] by blast
+      ultimately show "\<Gamma> \<turnstile> S1 \<rightarrow> S2 <: T" using top_case by blast
     next
-      case (S_All \<Gamma>1 X S1 S2 T1 T2) --{* lh drv.: @{term "\<Gamma>\<turnstile>S<:Q \<equiv> \<Gamma>1\<turnstile>\<forall>[X<:S1].S2 <: \<forall>[X<:T1].T2"} *} 
-      have lh_drv_prem1: "\<Gamma>1 \<turnstile> T1 <: S1" by fact
-      have lh_drv_prem2: "((X,T1)#\<Gamma>1) \<turnstile> S2 <: T2" by fact
-      have rh_deriv: "\<Gamma>1 \<turnstile> Q <: T" by fact
-      have fresh_cond: "X\<sharp>\<Gamma>1" "X\<sharp>S1" "X\<sharp>T1" by fact
-      have Q_inst: "\<forall>[X<:T1].T2 = Q" by fact
-      have measure: "size_ty T1 < size_ty Q" "size_ty T2 < size_ty Q " using Q_inst by force+
-      have "S1 closed_in \<Gamma>1" and "S2 closed_in ((X,T1)#\<Gamma>1)" 
-	using lh_drv_prem1 lh_drv_prem2 by (simp_all add: subtype_implies_closed)
-      hence "(\<forall>[X<:S1].S2) closed_in \<Gamma>1" by (force simp add: closed_in_def ty.supp abs_supp)
+      case (S_All \<Gamma> X S1 S2 Q1 Q2) 
+	--{* in this case lh drv is @{term "\<Gamma>\<turnstile>\<forall>[X<:S1].S2 <: \<forall>[X<:Q1].Q2"} *}
+      hence rh_drv: "\<Gamma> \<turnstile> \<forall>[X<:Q1].Q2 <: T" by simp
+      have lh_drv_prm1: "\<Gamma> \<turnstile> Q1 <: S1" by fact
+      have lh_drv_prm2: "((X,Q1)#\<Gamma>) \<turnstile> S2 <: Q2" by fact
+      have fresh_cond: "X\<sharp>\<Gamma>" "X\<sharp>Q1" by fact
+      have Q_inst: "\<forall>[X<:Q1].Q2 = Q" by fact
+      hence Q1_less: "size_ty Q1 < size_ty Q" 
+	and Q2_less: "size_ty Q2 < size_ty Q " by auto
+      have "S1 closed_in \<Gamma>" and "S2 closed_in ((X,Q1)#\<Gamma>)" 
+	using lh_drv_prm1 lh_drv_prm2 by (simp_all add: subtype_implies_closed)
+      hence "(\<forall>[X<:S1].S2) closed_in \<Gamma>" by (force simp add: closed_in_def ty.supp abs_supp)
       moreover
-      have "\<turnstile> \<Gamma>1 ok" using rh_deriv by (rule subtype_implies_ok)
+      have "\<turnstile> \<Gamma> ok" using rh_drv by (rule subtype_implies_ok)
       moreover
-        (* FIX: Maybe T3,T4 could be T1',T2' *)
-      have "T = Top \<or> (\<exists>T3 T4. T=\<forall>[X<:T3].T4 \<and> \<Gamma>1 \<turnstile> T3 <: T1 \<and> ((X,T3)#\<Gamma>1) \<turnstile> T2 <: T4)" 
-	using rh_deriv fresh_cond Q_inst by (auto dest: S_AllE_left simp add: fresh_prod)
+      from rh_drv have "T = Top \<or> (\<exists>T1 T2. T = \<forall>[X<:T1].T2 \<and> \<Gamma> \<turnstile> T1 <: Q1 \<and> ((X,T1)#\<Gamma>) \<turnstile> Q2 <: T2)" 
+	using fresh_cond by (simp add: S_AllE_left)
       moreover
-      { assume "\<exists>T3 T4. T=\<forall>[X<:T3].T4 \<and> \<Gamma>1 \<turnstile> T3 <: T1 \<and> ((X,T3)#\<Gamma>1) \<turnstile> T2 <: T4"
-	then obtain T3 T4 
-	  where T_inst: "T= \<forall>[X<:T3].T4" 
-	  and   rh_drv_prem1: "\<Gamma>1 \<turnstile> T3 <: T1" 
-	  and   rh_drv_prem2:"((X,T3)#\<Gamma>1) \<turnstile> T2 <: T4" by force
-        from IH1_outer[of "T1"] have "\<Gamma>1 \<turnstile> T3 <: S1" 
-	  using lh_drv_prem1 rh_drv_prem1 measure by blast
+      { assume "\<exists>T1 T2. T = \<forall>[X<:T1].T2 \<and> \<Gamma> \<turnstile> T1 <: Q1 \<and> ((X,T1)#\<Gamma>) \<turnstile> Q2 <: T2"
+	then obtain T1 T2 
+	  where T_inst: "T = \<forall>[X<:T1].T2" 
+	  and   rh_drv_prm1: "\<Gamma> \<turnstile> T1 <: Q1" 
+	  and   rh_drv_prm2:"((X,T1)#\<Gamma>) \<turnstile> Q2 <: T2" by force
+        from IH_trans[of "Q1"] have "\<Gamma> \<turnstile> T1 <: S1" 
+	  using lh_drv_prm1 rh_drv_prm1 Q1_less by blast
         moreover
-	from IH2_outer[of "T1"] have "((X,T3)#\<Gamma>1) \<turnstile> S2 <: T2" 
-	  using measure lh_drv_prem2 rh_drv_prem1 by force
-	with IH1_outer[of "T2"] have "((X,T3)#\<Gamma>1) \<turnstile> S2 <: T4" 
-	  using measure rh_drv_prem2 by force
+	from IH_narrow[of "Q1"] have "((X,T1)#\<Gamma>) \<turnstile> S2 <: Q2" 
+	  using Q1_less lh_drv_prm2 rh_drv_prm1 by blast
+	with IH_trans[of "Q2"] have "((X,T1)#\<Gamma>) \<turnstile> S2 <: T2" 
+	  using Q2_less rh_drv_prm2 by blast
         moreover
-	ultimately have "\<Gamma>1 \<turnstile> \<forall>[X<:S1].S2 <: T"
-	  using fresh_cond T_inst by (simp add: fresh_prod subtype_of_rel.S_All)
+	ultimately have "\<Gamma> \<turnstile> \<forall>[X<:S1].S2 <: \<forall>[X<:T1].T2"
+	  using fresh_cond by (simp add: subtype_of_rel.S_All)
+	hence "\<Gamma> \<turnstile> \<forall>[X<:S1].S2 <: T" using T_inst by simp
       }
-      ultimately show "\<Gamma>1 \<turnstile> \<forall>[X<:S1].S2 <: T" using Q_inst top_case[of "\<Gamma>1" "\<forall>[X<:S1].S2" _ "T'"] 
-	by auto
+      ultimately show "\<Gamma> \<turnstile> \<forall>[X<:S1].S2 <: T" using top_case by blast
     qed
   qed
 
+  --{* The inner induction for narrowing over @{term "(\<Delta>@[(X,Q)]@\<Gamma>) \<turnstile> M <: N"} *}
   have narrowing:
-    "\<And>\<Delta> \<Gamma> X M N P. (\<Delta>@(X,Q)#\<Gamma>) \<turnstile> M <: N \<Longrightarrow> \<Gamma> \<turnstile> P<:Q \<Longrightarrow> (\<Delta>@(X,P)#\<Gamma>) \<turnstile> M <: N"
+    "\<And>\<Delta> \<Gamma> X M N P. (\<Delta>@[(X,Q)]@\<Gamma>) \<turnstile> M <: N \<Longrightarrow> \<Gamma> \<turnstile> P<:Q \<Longrightarrow> (\<Delta>@[(X,P)]@\<Gamma>) \<turnstile> M <: N"
   proof -
-    fix \<Delta> \<Gamma> X M N P
-    assume a: "(\<Delta>@(X,Q)#\<Gamma>) \<turnstile> M <: N"
-    assume b: "\<Gamma> \<turnstile> P<:Q"
-    show "(\<Delta>@(X,P)#\<Gamma>) \<turnstile> M <: N"
-      using a b 
-    proof (nominal_induct \<Gamma>\<equiv>"\<Delta>@(X,Q)#\<Gamma>" M N avoiding: \<Delta> \<Gamma> X rule: subtype_of_rel_induct) 
-      case (S_Top \<Gamma>1 S1 \<Delta> \<Gamma>2 X)
-      then have lh_drv_prem1: "\<turnstile> (\<Delta>@(X,Q)#\<Gamma>2) ok" 
-           and  lh_drv_prem2: "S1 closed_in (\<Delta>@(X,Q)#\<Gamma>2)" by (simp_all only:)
-      have rh_drv: "\<Gamma>2 \<turnstile> P <: Q" by fact
-      hence "P closed_in \<Gamma>2" by (simp add: subtype_implies_closed)
-      with lh_drv_prem1 have "\<turnstile> (\<Delta>@(X,P)#\<Gamma>2) ok" by (simp only: replace_type)
+    fix \<Delta>' \<Gamma>' X M N P
+    assume a: "(\<Delta>'@[(X,Q)]@\<Gamma>') \<turnstile> M <: N"
+    assume b: "\<Gamma>' \<turnstile> P<:Q"
+    from a b show "(\<Delta>'@[(X,P)]@\<Gamma>') \<turnstile> M <: N" 
+    proof (nominal_induct \<Gamma>\<equiv>"\<Delta>'@[(X,Q)]@\<Gamma>'" M N avoiding: \<Delta>' \<Gamma>' X rule: subtype_of_rel_induct) 
+      case (S_Top _ S \<Delta> \<Gamma> X)
+	--{* in this case lh drv is @{term "(\<Delta>@[(X,Q)]@\<Gamma>) \<turnstile> S <: Top"} *}
+      hence lh_drv_prm1: "\<turnstile> (\<Delta>@[(X,Q)]@\<Gamma>) ok" 
+        and lh_drv_prm2: "S closed_in (\<Delta>@[(X,Q)]@\<Gamma>)" by simp_all
+      have rh_drv: "\<Gamma> \<turnstile> P <: Q" by fact
+      hence "P closed_in \<Gamma>" by (simp add: subtype_implies_closed)
+      with lh_drv_prm1 have "\<turnstile> (\<Delta>@[(X,P)]@\<Gamma>) ok" by (simp add: replace_type)
       moreover
-      from lh_drv_prem2 have "S1 closed_in (\<Delta>@(X,P)#\<Gamma>2)" by (simp add: closed_in_def domain_append)
-      ultimately show "(\<Delta>@(X,P)#\<Gamma>2) \<turnstile> S1 <: Top" by (rule subtype_of_rel.S_Top)
+      from lh_drv_prm2 have "S closed_in (\<Delta>@[(X,P)]@\<Gamma>)" by (simp add: closed_in_def domain_append)
+      ultimately show "(\<Delta>@[(X,P)]@\<Gamma>) \<turnstile> S <: Top" by (simp add: subtype_of_rel.S_Top)
     next
-      case (S_Var \<Gamma>1 X1 S1 T1 \<Delta> \<Gamma>2 X)
-      then have lh_drv_prem1: "\<turnstile> (\<Delta>@(X,Q)#\<Gamma>2) ok" 
-           and  lh_drv_prem2: "(X1,S1)\<in>set (\<Delta>@(X,Q)#\<Gamma>2)" 
-           and  lh_drv_prem3: "(\<Delta>@(X,Q)#\<Gamma>2) \<turnstile> S1 <: T1" 
-           and  IH_inner: "\<Gamma>2 \<turnstile> P <: Q \<Longrightarrow> (\<Delta>@(X,P)#\<Gamma>2) \<turnstile> S1 <: T1" by (simp_all only:)
-      have rh_drv: "\<Gamma>2 \<turnstile> P <: Q" by fact
-      hence "P closed_in \<Gamma>2" by (simp add: subtype_implies_closed)
-      hence a3: "\<turnstile> (\<Delta>@(X,P)#\<Gamma>2) ok" using lh_drv_prem1 by (simp only: replace_type)
-      show "(\<Delta>@(X,P)#\<Gamma>2) \<turnstile> TyVar X1 <: T1"
-      proof (cases "X=X1")
-	case False
-	have b0: "X\<noteq>X1" by fact
-	from lh_drv_prem3 rh_drv IH_inner 
-	have b1: "(\<Delta>@(X,P)#\<Gamma>2) \<turnstile> S1 <: T1" by simp
-	from lh_drv_prem2 b0 have b2: "(X1,S1)\<in>set (\<Delta>@(X,P)#\<Gamma>2)" by simp
-	show "(\<Delta>@(X,P)#\<Gamma>2) \<turnstile> TyVar X1 <: T1" using a3 b2 b1 by (rule subtype_of_rel.S_Var)
-      next 
-	case True
-	have b0: "X=X1" by fact
-	have a4: "S1=Q"
-	proof -
-	  have "(X1,Q)\<in>set (\<Delta>@(X,Q)#\<Gamma>2)" using b0 by simp
-	  with lh_drv_prem1 lh_drv_prem2 show "S1=Q" by (blast intro: uniqueness_of_ctxt)
-	qed
-	have a5: "(\<Delta>@(X,P)#\<Gamma>2) extends \<Gamma>2" by (force simp add: extends_def)
-	have a6: "(\<Delta>@(X1,P)#\<Gamma>2) \<turnstile> P <: Q" using b0 a5 rh_drv a3 by (simp add: weakening)	
-	have a7: "(\<Delta>@(X1,P)#\<Gamma>2) \<turnstile> Q <: T1" using b0 IH_inner lh_drv_prem3 rh_drv a4 by simp
-	have a8: "(\<Delta>@(X1,P)#\<Gamma>2) \<turnstile> P <: T1" using a6 a7 transitivity by blast
-	have a9: "(X1,P)\<in>set (\<Delta>@(X,P)#\<Gamma>2)" using b0 by simp
-	show "(\<Delta>@(X,P)#\<Gamma>2) \<turnstile> TyVar X1 <: T1" using a3 b0 a8 a9 by force
-      qed
+      case (S_Var _ Y S N \<Delta> \<Gamma> X) 
+	--{* in this case lh drv is @{term "(\<Delta>@[(X,Q)]@\<Gamma>) \<turnstile> TVar Y <: N"} *}
+      hence IH_inner: "(\<Delta>@[(X,P)]@\<Gamma>) \<turnstile> S <: N" 
+	and lh_drv_prm1: "\<turnstile> (\<Delta>@[(X,Q)]@\<Gamma>) ok" 
+        and lh_drv_prm2: "(Y,S)\<in>set (\<Delta>@[(X,Q)]@\<Gamma>)" by simp_all
+      have rh_drv: "\<Gamma> \<turnstile> P <: Q" by fact
+      hence "P closed_in \<Gamma>" by (simp add: subtype_implies_closed)
+      hence cntxt_ok: "\<turnstile> (\<Delta>@[(X,P)]@\<Gamma>) ok" using lh_drv_prm1 by (simp add: replace_type)
+	-- {* we distinguishing the cases @{term "X\<noteq>Y"} and @{term "X=Y"} (the latter 
+	being the interesting one) *}
+      { assume "X\<noteq>Y"
+	hence "(Y,S)\<in>set (\<Delta>@[(X,P)]@\<Gamma>)" using lh_drv_prm2 by simp
+	with IH_inner have "(\<Delta>@[(X,P)]@\<Gamma>) \<turnstile> TVar Y <: N" 
+	  using cntxt_ok by (simp add: subtype_of_rel.S_Var)
+      }
+      moreover
+      { have memb_XQ: "(X,Q)\<in>set (\<Delta>@[(X,Q)]@\<Gamma>)" by simp
+	have memb_XP: "(X,P)\<in>set (\<Delta>@[(X,P)]@\<Gamma>)" by simp
+	assume "X=Y" 
+	hence "S=Q" using lh_drv_prm1 lh_drv_prm2 memb_XQ by (simp only: uniqueness_of_ctxt)
+	hence "(\<Delta>@[(X,P)]@\<Gamma>) \<turnstile> Q <: N" using IH_inner by simp
+	moreover
+	have "(\<Delta>@[(X,P)]@\<Gamma>) extends \<Gamma>" by (simp add: extends_def)
+	hence "(\<Delta>@[(X,P)]@\<Gamma>) \<turnstile> P <: Q" using rh_drv cntxt_ok by (simp only: weakening)
+	ultimately have "(\<Delta>@[(X,P)]@\<Gamma>) \<turnstile> P <: N" using transitivity by simp
+	hence "(\<Delta>@[(X,P)]@\<Gamma>) \<turnstile> TVar X <: N" using memb_XP cntxt_ok 
+	  by (simp only: subtype_of_rel.S_Var)
+      }
+      ultimately show "(\<Delta>@[(X,P)]@\<Gamma>) \<turnstile> TVar Y <: N" by blast
     next
-      case (S_Refl \<Gamma>1 X1 \<Delta> \<Gamma>2 X)
-      have lh_drv_prem1: "\<turnstile> \<Gamma>1 ok" by fact
-      have lh_drv_prem2: "X1 \<in> domain \<Gamma>1" by fact
-      have \<Gamma>1_inst: "\<Gamma>1 = \<Delta>@(X,Q)#\<Gamma>2" by fact
-      have "\<Gamma>2 \<turnstile> P <: Q" by fact
-      hence "P closed_in \<Gamma>2" by (simp add: subtype_implies_closed)
-      hence a3: "\<turnstile> (\<Delta>@(X,P)#\<Gamma>2) ok" using lh_drv_prem1 \<Gamma>1_inst by (simp add: replace_type)
-      have b0: "X1 \<in> domain (\<Delta>@(X,P)#\<Gamma>2)" using lh_drv_prem2 \<Gamma>1_inst by (simp add: domain_append)
-      show "(\<Delta>@(X,P)#\<Gamma>2) \<turnstile> TyVar X1 <: TyVar X1" using a3 b0 by (rule subtype_of_rel.S_Refl)
+      case (S_Refl _ Y \<Delta> \<Gamma> X)
+	--{* in this case lh drv is @{term "(\<Delta>@[(X,Q)]@\<Gamma>) \<turnstile> TVar Y <: TVar Y"} *}
+      hence lh_drv_prm1: "\<turnstile> (\<Delta>@[(X,Q)]@\<Gamma>) ok" 
+	and lh_drv_prm2: "Y \<in> domain (\<Delta>@[(X,Q)]@\<Gamma>)" by simp_all
+      have "\<Gamma> \<turnstile> P <: Q" by fact
+      hence "P closed_in \<Gamma>" by (simp add: subtype_implies_closed)
+      with lh_drv_prm1 have "\<turnstile> (\<Delta>@[(X,P)]@\<Gamma>) ok" by (simp add: replace_type)
+      moreover
+      from lh_drv_prm2 have "Y \<in> domain (\<Delta>@[(X,P)]@\<Gamma>)" by (simp add: domain_append)
+      ultimately show "(\<Delta>@[(X,P)]@\<Gamma>) \<turnstile> TVar Y <: TVar Y" by (simp add: subtype_of_rel.S_Refl)
     next
-      case S_Arrow thus ?case by blast
+      case (S_Arrow _ Q1 Q2 S1 S2 \<Delta> \<Gamma> X) 
+	--{* in this case lh drv is @{term "(\<Delta>@[(X,Q)]@\<Gamma>) \<turnstile> Q1 \<rightarrow> Q2 <: S1 \<rightarrow> S2"} *}
+      thus "(\<Delta>@[(X,P)]@\<Gamma>) \<turnstile> Q1 \<rightarrow> Q2 <: S1 \<rightarrow> S2" by blast 
     next
-      case (S_All \<Gamma>1 X1 S1 S2 T1 T2 \<Delta> \<Gamma>2 X)
-      have IH_inner1: "\<And>\<Delta> \<Gamma> X. \<Gamma> \<turnstile> P <: Q \<Longrightarrow> \<Gamma>1 = \<Delta>@(X,Q)#\<Gamma> \<Longrightarrow> (\<Delta>@(X,P)#\<Gamma>) \<turnstile> T1 <: S1" by fact
-      have IH_inner2: "\<And>\<Delta> \<Gamma> X. \<Gamma> \<turnstile> P <: Q \<Longrightarrow> (X1,T1)#\<Gamma>1 = \<Delta>@(X,Q)#\<Gamma> \<Longrightarrow> (\<Delta>@(X,P)#\<Gamma>) \<turnstile> S2 <: T2" 
-	by fact
-      have lh_drv_prem1: "\<Gamma>1 \<turnstile> T1 <: S1" by fact
-      have lh_drv_prem2: "X1\<sharp>\<Gamma>1" "X1\<sharp>S1" "X1\<sharp>T1" by fact (* check this whether this is the lh_drv_p2 *)
-      have lh_drv_prem3: "((X1,T1)#\<Gamma>1) \<turnstile> S2 <: T2" by fact
-      have \<Gamma>1_inst: "\<Gamma>1 = \<Delta>@(X,Q)#\<Gamma>2" by fact
-      have a2: "\<Gamma>2 \<turnstile> P <: Q" by fact
-      have b0: "(\<Delta>@(X,P)#\<Gamma>2) \<turnstile> T1 <: S1" using \<Gamma>1_inst a2 lh_drv_prem1 IH_inner1 by simp
-      have b1: "(((X1,T1)#\<Delta>)@(X,P)#\<Gamma>2) \<turnstile> S2 <: T2" using \<Gamma>1_inst a2 lh_drv_prem3 IH_inner2
-	apply(auto)
-	apply(drule_tac x="\<Gamma>2" in meta_spec)
-	apply(drule_tac x="(X1,T1)#\<Delta>" in meta_spec)
-	apply(auto)
-	done
-      have b3: "X1\<sharp>(\<Delta>@(X,P)#\<Gamma>2)" using lh_drv_prem2 \<Gamma>1_inst a2
-	by (auto simp add: fresh_prod fresh_list_append fresh_list_cons dest: subtype_implies_fresh)
-      show "(\<Delta>@(X,P)#\<Gamma>2) \<turnstile> \<forall> [X1<:S1].S2 <: \<forall> [X1<:T1].T2" using b0 b3 b1 by force 
+      case (S_All _ Y S1 S2 T1 T2 \<Delta> \<Gamma> X)
+	--{* in this case lh drv is @{term "(\<Delta>@[(X,Q)]@\<Gamma>) \<turnstile> \<forall>[Y<:S1].S2 <: \<forall>[Y<:T1].T2"} *}
+      hence IH_inner1: "(\<Delta>@[(X,P)]@\<Gamma>) \<turnstile> T1 <: S1" 
+	and IH_inner2: "((Y,T1)#\<Delta>@[(X,P)]@\<Gamma>) \<turnstile> S2 <: T2" 
+	and lh_drv_prm2: "Y\<sharp>(\<Delta>@[(X,Q)]@\<Gamma>)" by force+
+      have rh_drv: "\<Gamma> \<turnstile> P <: Q" by fact
+      hence "Y\<sharp>P" using lh_drv_prm2 by (simp only: fresh_list_append subtype_implies_fresh)
+      hence "Y\<sharp>(\<Delta>@[(X,P)]@\<Gamma>)" using lh_drv_prm2 
+	by (simp add: fresh_list_append fresh_list_cons fresh_prod)
+      with IH_inner1 IH_inner2 
+      show "(\<Delta>@[(X,P)]@\<Gamma>) \<turnstile> \<forall>[Y<:S1].S2 <: \<forall>[Y<:T1].T2" by (simp add: subtype_of_rel.S_All)
     qed
   qed
   from transitivity narrowing show ?case by blast 
 qed
 
 
- 
-section {* Terms *}
 
-nominal_datatype trm = Var   "vrs"
-                     | Lam   "\<guillemotleft>vrs\<guillemotright>trm" "ty"
-                     | TAbs  "\<guillemotleft>tyvrs\<guillemotright>trm" "ty"
-                     | App   "trm" "trm"
-                     | TApp  "trm" "ty"
-
-consts
-  Lam_syn   :: "vrs \<Rightarrow> ty \<Rightarrow> trm \<Rightarrow> trm"   ("Lam [_:_]._" [100,100,100] 100)
-  TAbs_syn  :: "tyvrs \<Rightarrow> ty \<Rightarrow> trm \<Rightarrow> trm" ("TAbs [_<:_]._" [100,100,100] 100)
-translations 
-  "Lam  [a:tys].t" \<rightleftharpoons> "trm.Lam a t tys"
-  "TAbs [a<:tys].t" \<rightleftharpoons> "trm.TAbs a t tys"
 
 end
